commitment in progress

proof/rejection_sampling/Ops_LeakageAnalysis.ec
@@ -87,3 +87,94 @@ simplify. smt(). smt(). rewrite /set0_f. rewrite (set0_g_comp_2 (i{hr} +1)).  sm
 skip. progress. rewrite /set0_f.  rewrite set0_g_comp_1. auto. auto. 
 smt().
 qed.
+
+
+(* set1 LEAKAGES  *)
+op set1_prefix : leakages_t = LeakFor (1, 32) :: LeakAddr [] :: LeakAddr [0] :: LeakAddr [] :: [].
+op set1_step (i : int) : leakages_t = LeakAddr [i] :: LeakAddr [] :: [].
+
+op set1_g (x : int) : leakages_t.
+axiom set1_g_comp_1 x : x <= 1 => set1_g x = [].
+axiom set1_g_comp_2 x : 1 <  x => set1_g x = set1_step (x-1) ++ set1_g (x - 1).
+
+op set1_f (x : int) : leakages_t = set1_g x ++ set1_prefix.
+
+lemma bn_set1_leakages start_l :
+   hoare [ M(Syscall).bn_set1 : M.leakages = start_l 
+                ==> M.leakages = set1_f 32 ++ start_l ].
+proof. 
+proc.
+sp.  elim*. progress.
+conseq (_: M.leakages = set1_prefix ++ start_l /\ i = 1 ==> _).
+progress. rewrite /set1_prefix.
+while (1 <= i /\ i <= 32 /\ M.leakages = set1_f i ++ start_l).
+wp.  skip.  progress. 
+simplify. smt(). smt(). rewrite /set1_f.  simplify. rewrite (set1_g_comp_2 (i{hr} + 1)).  smt(). simplify. rewrite /set1_step. simplify. auto.
+skip. 
+progress.  rewrite /set1_f.  rewrite set1_g_comp_1. auto. auto. 
+smt().
+qed.
+
+(* ith_bit64 leakages  *)
+op ith_bit64_t : leakages_t = LeakAddr [] :: LeakAddr [] :: LeakAddr [] :: LeakAddr [] :: LeakAddr [] :: [].
+
+lemma ith_bit64_leakages start_l :
+   hoare [ M(Syscall).ith_bit64 : M.leakages = start_l 
+                ==> M.leakages = ith_bit64_t ++ start_l ].
+proc. wp. skip. progress. qed.
+
+(* ith_bit LEAKAGES  *)
+op ith_bit_t (x : W64.t) :  leakages_t = 
+ ith_bit64_t ++ LeakAddr [] :: LeakAddr [to_uint (x `>>` (of_int 6)%W8)] :: LeakAddr [] ::  LeakAddr [] :: LeakAddr [] :: LeakAddr [] :: [].
+
+lemma ith_bit_leakages start_l c :
+   hoare [ M(Syscall).ith_bit : M.leakages = start_l /\ c = ctr 
+                ==> M.leakages = ith_bit_t c ++ start_l ].
+proof. 
+proc.
+wp. 
+sp. elim*. progress. 
+exists* c1. elim*. move => c1_var.
+call (ith_bit64_leakages (LeakAddr [] :: LeakAddr [to_uint  c1_var   ] :: LeakAddr [] :: LeakAddr [] :: 
+  LeakAddr [] :: LeakAddr [] :: start_l)).
+skip. progress. 
+qed.
+
+
+(* swapr LEAKAGES  *)
+op swapr_prefix : leakages_t = LeakFor (0, 32) :: LeakAddr [] :: LeakAddr [] :: [].
+op swapr_step (x : int) : leakages_t = LeakAddr [x] :: LeakAddr [] :: LeakAddr [] :: LeakAddr [x] :: 
+LeakAddr [x] :: LeakAddr [x] :: LeakAddr [] :: LeakAddr [x] :: 
+LeakAddr [x] :: [].
+
+op swapr_g (x : int) : leakages_t.
+axiom swapr_g_comp_1 x : x = 0 => swapr_g x = [].
+axiom swapr_g_comp_2 x : 0 <  x => swapr_g x = swapr_step (x-1) ++ swapr_g (x - 1).
+
+op swapr_f (x : int) : leakages_t = swapr_g x ++ swapr_prefix.
+
+lemma swapr_leakages start_l :
+   hoare [ M(Syscall).swapr : M.leakages = start_l 
+     ==> M.leakages = swapr_f 32 ++ start_l ].
+proof. 
+proc.
+sp.  elim*. progress.
+conseq (_: M.leakages = swapr_prefix ++ start_l /\ i = 0 ==> _).
+progress.
+while (0 <= i /\ i <= 32 /\ M.leakages = swapr_f i ++ start_l).
+wp.  skip.  progress. 
+smt(). smt(). 
+rewrite /swapr_f. rewrite (swapr_g_comp_2 (i{hr} +1)).  smt(). simplify. rewrite /swapr_step. simplify. auto.
+skip. progress. rewrite /swapr_f.  rewrite swapr_g_comp_1. auto. auto. 
+smt().
+qed.
+
+
+(* mulm LEAKAGES  *)
+op mulm_t :  leakages_t.
+
+lemma mulm_leakages start_l :
+   hoare [ M(Syscall).mulm : M.leakages = start_l 
+                ==> M.leakages = mulm_t ++ start_l ].
+admitted.
+
